dist/gcc-compatible/Hacl_MAC_Poly1305_Simd128.c
@@ -1304,6 +1304,11 @@ Hacl_MAC_Poly1305_Simd128_poly1305_finish(
 Hacl_MAC_Poly1305_Simd128_state_t *Hacl_MAC_Poly1305_Simd128_malloc(uint8_t *key)
 {
   uint8_t *buf = (uint8_t *)KRML_HOST_CALLOC(32U, sizeof (uint8_t));
+  if (buf == NULL)
+  {
+    return NULL;
+  }
+  uint8_t *buf1 = buf;
   Lib_IntVector_Intrinsics_vec128
   *r1 =
     (Lib_IntVector_Intrinsics_vec128 *)KRML_ALIGNED_MALLOC(16,
@@ -1314,13 +1319,20 @@ Hacl_MAC_Poly1305_Simd128_state_t *Hacl_MAC_Poly1305_Simd128_malloc(uint8_t *key
   memcpy(k_, key, 32U * sizeof (uint8_t));
   uint8_t *k_0 = k_;
   Hacl_MAC_Poly1305_Simd128_state_t
-  s = { .block_state = block_state, .buf = buf, .total_len = (uint64_t)0U, .p_key = k_0 };
+  s = { .block_state = block_state, .buf = buf1, .total_len = (uint64_t)0U, .p_key = k_0 };
   Hacl_MAC_Poly1305_Simd128_state_t
   *p =
     (Hacl_MAC_Poly1305_Simd128_state_t *)KRML_HOST_MALLOC(sizeof (
         Hacl_MAC_Poly1305_Simd128_state_t
       ));
   p[0U] = s;
+  if (p == NULL)
+  {
+    KRML_HOST_FREE(k_0);
+    KRML_ALIGNED_FREE(block_state);
+    KRML_HOST_FREE(buf1);
+    return NULL;
+  }
   Hacl_MAC_Poly1305_Simd128_poly1305_init(block_state, key);
   return p;
 }
