code/streaming/Hacl.Streaming.Functor.fst
@@ -275,6 +275,13 @@ let seen_length #index c i t t' s =
   let State _ _ total_len _ _ = !*s in
   total_len
 
+(* as far as I know, we are the only clients of LowStar.Monotonic.Buffer who
+ * care about catching potential allocation failures, meaning this abbreviation was
+ * never defined in the standard F* library -- should be done at some point, I
+ * guess *)
+inline_for_extraction noextract
+let fallible_malloc #a = LowStar.Monotonic.Buffer.(mmalloc_partial #a #(LowStar.Buffer.trivial_preorder a))
+
 (* TODO: malloc and alloca have big portions of proofs in common, so it may
  * be possible to factorize them, but it is not clear how *)
 #restart-solver
@@ -287,98 +294,124 @@ let malloc #index c i t t' key r =
   (**) let h0 = ST.get () in
 
   (**) B.loc_unused_in_not_unused_in_disjoint h0;
-  let buf = B.malloc r (Lib.IntTypes.u8 0) (c.blocks_state_len i) in
-  (**) let h1 = ST.get () in
-  (**) assert (B.fresh_loc (B.loc_buffer buf) h0 h1);
-  (**) B.loc_unused_in_not_unused_in_disjoint h1;
-  (**) B.(modifies_only_not_unused_in loc_none h0 h1);
-  (**) c.key.frame_invariant B.loc_none key h0 h1;
+  let buf = fallible_malloc r (Lib.IntTypes.u8 0) (c.blocks_state_len i) in
+  if B.is_null buf then
+    B.null
+  else
+    (**) let h1 = ST.get () in
+    assert (LowStar.Monotonic.Buffer.frameOf buf == r);
+    assert (LowStar.Monotonic.Buffer.freeable buf);
+    assert (LowStar.Monotonic.Buffer.alloc_post_mem_common buf h0 h1
+      (Seq.create (U32.v (c.blocks_state_len i)) (Lib.IntTypes.u8 0)));
+    let buf: LowStar.Monotonic.Buffer.lmbuffer uint8 (LowStar.Buffer.trivial_preorder uint8)
+      (LowStar.Buffer.trivial_preorder uint8) (U32.v (c.blocks_state_len i)) = buf in
+    (**) assert (B.fresh_loc (B.loc_buffer buf) h0 h1);
+    (**) B.loc_unused_in_not_unused_in_disjoint h1;
+    (**) B.(modifies_only_not_unused_in loc_none h0 h1);
+    (**) c.key.frame_invariant B.loc_none key h0 h1;
 
-  let block_state = c.state.create_in i r in
-  (**) let h2 = ST.get () in
-  (**) assert (B.fresh_loc (c.state.footprint #i h2 block_state) h0 h2);
-  (**) B.loc_unused_in_not_unused_in_disjoint h2;
-  (**) B.(modifies_only_not_unused_in loc_none h1 h2);
-  (**) c.key.frame_invariant B.loc_none key h1 h2;
+    let block_state = c.state.create_in i r in
+    (**) let h2 = ST.get () in
+    (**) assert (B.fresh_loc (c.state.footprint #i h2 block_state) h0 h2);
+    (**) B.loc_unused_in_not_unused_in_disjoint h2;
+    (**) B.(modifies_only_not_unused_in loc_none h1 h2);
+    (**) c.key.frame_invariant B.loc_none key h1 h2;
 
-  let k': optional_key i c.km c.key =
-    match c.km with
-    | Runtime ->
-        let k' = c.key.create_in i r in
-        (**) let h3 = ST.get () in
-        (**) B.loc_unused_in_not_unused_in_disjoint h3;
-        (**) B.(modifies_only_not_unused_in loc_none h2 h3);
-        (**) c.key.frame_invariant B.loc_none key h2 h3;
-        (**) c.state.frame_invariant B.loc_none block_state h2 h3;
-        (**) c.state.frame_freeable B.loc_none block_state h2 h3;
-        (**) assert (B.fresh_loc (c.key.footprint #i h3 k') h0 h3);
-        (**) assert (c.key.invariant #i h3 k');
-        (**) assert (c.key.invariant #i h3 key);
-        (**) assert B.(loc_disjoint (c.key.footprint #i h3 key) (c.key.footprint #i h3 k'));
-        c.key.copy i key k';
-        (**) let h4 = ST.get () in
-        (**) assert (B.fresh_loc (c.key.footprint #i h4 k') h0 h4);
-        (**) B.loc_unused_in_not_unused_in_disjoint h4;
-        (**) B.(modifies_only_not_unused_in loc_none h2 h4);
-        (**) assert (c.key.invariant #i h4 k');
-        (**) c.key.frame_invariant (c.key.footprint #i h3 k') key h3 h4;
-        (**) c.state.frame_invariant (c.key.footprint #i h3 k') block_state h3 h4;
-        (**) c.state.frame_freeable (c.key.footprint #i h3 k') block_state h3 h4;
-        k'
-    | Erased ->
-        G.hide (c.key.v i h0 key)
-  in
-  (**) let h5 = ST.get () in
-  (**) assert (B.fresh_loc (optional_footprint h5 k') h0 h5);
-  (**) assert (B.fresh_loc (c.state.footprint #i h5 block_state) h0 h5);
+    let k': optional_key i c.km c.key =
+      match c.km with
+      | Runtime ->
+          let k' = c.key.create_in i r in
+          (**) let h3 = ST.get () in
+          (**) B.loc_unused_in_not_unused_in_disjoint h3;
+          (**) B.(modifies_only_not_unused_in loc_none h2 h3);
+          (**) c.key.frame_invariant B.loc_none key h2 h3;
+          (**) c.state.frame_invariant B.loc_none block_state h2 h3;
+          (**) c.state.frame_freeable B.loc_none block_state h2 h3;
+          (**) assert (B.fresh_loc (c.key.footprint #i h3 k') h0 h3);
+          (**) assert (c.key.invariant #i h3 k');
+          (**) assert (c.key.invariant #i h3 key);
+          (**) assert B.(loc_disjoint (c.key.footprint #i h3 key) (c.key.footprint #i h3 k'));
+          c.key.copy i key k';
+          (**) let h4 = ST.get () in
+          (**) assert (B.fresh_loc (c.key.footprint #i h4 k') h0 h4);
+          (**) B.loc_unused_in_not_unused_in_disjoint h4;
+          (**) B.(modifies_only_not_unused_in loc_none h2 h4);
+          (**) assert (c.key.invariant #i h4 k');
+          (**) c.key.frame_invariant (c.key.footprint #i h3 k') key h3 h4;
+          (**) c.state.frame_invariant (c.key.footprint #i h3 k') block_state h3 h4;
+          (**) c.state.frame_freeable (c.key.footprint #i h3 k') block_state h3 h4;
+          k'
+      | Erased ->
+          G.hide (c.key.v i h0 key)
+    in
+    (**) let h5 = ST.get () in
+    (**) assert (B.fresh_loc (optional_footprint h5 k') h0 h5);
+    (**) assert (B.fresh_loc (c.state.footprint #i h5 block_state) h0 h5);
 
-  [@inline_let] let total_len = Int.Cast.uint32_to_uint64 (c.init_input_len i) in
-  let s = State block_state buf total_len (G.hide S.empty) k' in
-  (**) assert (B.fresh_loc (footprint_s c i h5 s) h0 h5);
+    [@inline_let] let total_len = Int.Cast.uint32_to_uint64 (c.init_input_len i) in
+    let s = State block_state buf total_len (G.hide S.empty) k' in
+    (**) assert (B.fresh_loc (footprint_s c i h5 s) h0 h5);
 
-  (**) B.loc_unused_in_not_unused_in_disjoint h5;
-  let p = B.malloc r s 1ul in
-  (**) let h6 = ST.get () in
-  (**) B.(modifies_only_not_unused_in loc_none h5 h6);
-  (**) B.(modifies_only_not_unused_in loc_none h0 h6);
-  (**) c.key.frame_invariant B.loc_none key h5 h6;
-  (**) c.state.frame_invariant B.loc_none block_state h5 h6;
-  (**) optional_frame B.loc_none k' h5 h6;
-  (**) assert (B.fresh_loc (B.loc_addr_of_buffer p) h0 h6);
-  (**) assert (B.fresh_loc (footprint_s c i h6 s) h0 h6);
-  (**) c.state.frame_freeable B.loc_none block_state h5 h6;
-  (**) assert (optional_reveal h5 k' == optional_reveal h6 k');
+    (**) B.loc_unused_in_not_unused_in_disjoint h5;
+    let p = fallible_malloc r s 1ul in
+    if B.is_null p then begin
+      begin match c.km with
+      | Runtime ->
+          let h6 = ST.get () in
+          c.key.free i k';
+          let h7 = ST.get () in
+          (**) c.state.frame_invariant (c.key.footprint #i h6 k') block_state h6 h7;
+          (**) c.state.frame_freeable (c.key.footprint #i h6 k') block_state h6 h7;
+          (**) B.(modifies_only_not_unused_in loc_none h0 h7)
+      | _ -> ()
+      end;
+      c.state.free i block_state;
+      B.free buf;
+      let h8 = ST.get () in
+      (**) B.(modifies_only_not_unused_in loc_none h0 h8);
+      B.null
+    end else
+      (**) let h6 = ST.get () in
+      (**) B.(modifies_only_not_unused_in loc_none h5 h6);
+      (**) B.(modifies_only_not_unused_in loc_none h0 h6);
+      (**) c.key.frame_invariant B.loc_none key h5 h6;
+      (**) c.state.frame_invariant B.loc_none block_state h5 h6;
+      (**) optional_frame B.loc_none k' h5 h6;
+      (**) assert (B.fresh_loc (B.loc_addr_of_buffer p) h0 h6);
+      (**) assert (B.fresh_loc (footprint_s c i h6 s) h0 h6);
+      (**) c.state.frame_freeable B.loc_none block_state h5 h6;
+      (**) assert (optional_reveal h5 k' == optional_reveal h6 k');
 
-  c.init (G.hide i) key buf block_state;
-  (**) let h7 = ST.get () in
-  (**) assert (B.fresh_loc (c.state.footprint #i h7 block_state) h0 h7);
-  (**) assert (B.fresh_loc (B.loc_buffer buf) h0 h7);
-  (**) optional_frame (B.loc_union (c.state.footprint #i h7 block_state) (B.loc_buffer buf)) k' h6 h7;
-  (**) c.update_multi_zero i (c.state.v i h7 block_state) 0;
-  (**) B.modifies_only_not_unused_in B.loc_none h0 h7;
-  (**) assert (c.state.v i h7 block_state == c.init_s i (optional_reveal h6 k'));
+      c.init (G.hide i) key buf block_state;
+      (**) let h7 = ST.get () in
+      (**) assert (B.fresh_loc (c.state.footprint #i h7 block_state) h0 h7);
+      (**) assert (B.fresh_loc (B.loc_buffer buf) h0 h7);
+      (**) optional_frame (B.loc_union (c.state.footprint #i h7 block_state) (B.loc_buffer buf)) k' h6 h7;
+      (**) c.update_multi_zero i (c.state.v i h7 block_state) 0;
+      (**) B.modifies_only_not_unused_in B.loc_none h0 h7;
+      (**) assert (c.state.v i h7 block_state == c.init_s i (optional_reveal h6 k'));
 
-  (**) let h8 = ST.get () in
-  (**) assert (U64.v total_len <= U64.v (c.max_input_len i));
+      (**) let h8 = ST.get () in
+      (**) assert (U64.v total_len <= U64.v (c.max_input_len i));
 
-  (**) begin
-  (**) let s = B.get h8 p 0 in
-  (**) let key_v = reveal_key c i h8 p in
-  (**) let init_input = c.init_input_s i key_v in
-  (**) split_at_last_init c i init_input;
-  (**) assert(invariant_s c i h8 s)
-  (**) end;
-  (**) assert (invariant c i h8 p);
+      (**) begin
+      (**) let s = B.get h8 p 0 in
+      (**) let key_v = reveal_key c i h8 p in
+      (**) let init_input = c.init_input_s i key_v in
+      (**) split_at_last_init c i init_input;
+      (**) assert(invariant_s c i h8 s)
+      (**) end;
+      (**) assert (invariant c i h8 p);
 
-  (**) assert (seen c i h8 p == S.empty);
-  (**) assert B.(modifies loc_none h0 h8);
-  (**) assert (B.fresh_loc (footprint c i h8 p) h0 h8);
-  (**) assert B.(loc_includes (loc_region_only true r) (footprint c i h8 p));
+      (**) assert (seen c i h8 p == S.empty);
+      (**) assert B.(modifies loc_none h0 h8);
+      (**) assert (B.fresh_loc (footprint c i h8 p) h0 h8);
+      (**) assert B.(loc_includes (loc_region_only true r) (footprint c i h8 p));
 
-  (**) assert (ST.equal_stack_domains h1 h8);
-  (**) assert (ST.equal_stack_domains h0 h1);
+      (**) assert (ST.equal_stack_domains h1 h8);
+      (**) assert (ST.equal_stack_domains h0 h1);
 
-  p
+      p
 #pop-options
 
 #push-options "--z3rlimit 100"
